Implement symbol allocation.

test.v
@@ -9,6 +9,7 @@ From iris.heap_lang Require Import primitive_laws.
 From iris.base_logic.lib Require Import invariants.
 Import uPred.
 
+
 Definition specN := nroot .@ "spec".
 
 (** The CMRA for the heap of the specification. *)
@@ -452,3 +453,466 @@ Section cfg.
     eapply rtc_r, step_insert; eauto. econstructor; eauto.
   Qed.
 End cfg.
+
+Definition perm `{!EqDecision T, !Countable T} (X : gset (T * T)) :=
+  forall p1 p2, p1 ∈ X → p2 ∈ X → (p1.1 = p1.2 ↔ p2.1 = p2.2).
+
+Class symbolSG Σ := SymbolSG {
+  symbol_inG :> inG Σ (authR (gsetUR (prodO locO locO)))
+}.
+
+Section Symbol.
+
+Context `{!heapG Σ, !cfgSG Σ, !symbolSG Σ}.
+
+Implicit Types γ : gname.
+Implicit Types LL : gsetUR (prodO locO locO).
+Implicit Types l : loc.
+Implicit Types v : val.
+
+Definition symbols γ : iProp Σ :=
+  ∃ LL, own γ (● LL) ∗ [∗ set] ll ∈ LL, ll.1 ↦ #() ∗ ll.2 ↦ₛ #().
+
+Definition symbol γ v1 v2 : iProp Σ :=
+  ∃ l1 l2, ⌜v1 = #l1⌝ ∗ ⌜v2 = #l2⌝ ∗ own γ (◯ {[l1, l2]}).
+
+Lemma persistent_symbol γ v1 v2 : Persistent (symbol γ v1 v2).
+Proof. apply _. Qed.
+
+Definition mksymbol : val := λ: <>, ref #().
+
+Lemma wp_mksymbol γ j K :
+  spec_ctx -∗
+  symbols γ -∗
+  j ⤇ fill K (mksymbol #()%V) -∗
+  WP mksymbol #()%V {{ v1, ∃ v2, symbol γ v1 v2 ∗ j ⤇ fill K v2}}.
+Proof.
+rewrite /symbols /mksymbol.
+iIntros "#Hinv"; iDestruct 1 as (LL) "[Hown Hlocs]"; iIntros "Hspec".
+iPoseProof (step_lam ⊤ with "[Hinv Hspec]") as "> Hspec"; first done.
+  by iSplit.
+rewrite /=.
+iPoseProof (step_alloc ⊤ with "[Hinv Hspec]") as "> Hspec"; first done.
+  by iSplit.
+iDestruct "Hspec" as (l2) "[Hspec Hl2]".
+iApply wp_fupd; wp_pures; wp_alloc l1 as "Hl1".
+pose (Fl := ◯ {[l1, l2]}).
+iMod (own_update _ _ (● (LL ⋅ {[l1, l2]}) ⋅ Fl) with "Hown") as "Hown".
+  etrans.
+  - eapply auth_update_auth.
+    by apply gset_local_update, union_subseteq_l.
+  - apply auth_update_core_id.
+    + by apply gset_core_id.
+    + by apply gset_included, union_subseteq_r.
+rewrite own_op; iDestruct "Hown" as "[Hown Hl1l2]".
+iModIntro; iExists #l2; iSplit=> //.
+iExists l1, l2; do !iSplit; eauto.
+Qed.
+
+Lemma symbols_alloc : ⊢ |==> ∃ γ, symbols γ.
+Proof.
+iMod (own_alloc (● ∅ : auth (gset (loc * loc)))) as (γ) "Hown".
+  by apply/auth_auth_valid.
+by iModIntro; iExists γ, ∅; iFrame.
+Qed.
+
+End Symbol.
+
+Inductive term  :=
+| TInt of Z
+| TPair of term & term
+| TNonce of loc
+| TKey of loc
+| TEnc of loc & term.
+
+Fixpoint val_of_term t : val :=
+  match t with
+  | TInt n => (#0, #n)
+  | TPair t1 t2 => (#1, (val_of_term t1, val_of_term t2))%V
+  | TNonce l => (#2, #l)%V
+  | TKey l => (#3, #l)%V
+  | TEnc l t => (#4, (#l, val_of_term t))
+  end.
+
+
+
+
+
+
+
+Class keysSG Σ := KeysSG {
+  keys_inG  :> inG Σ (authR (gsetUR (prodO boolO locO)));
+  keys_inG2 :> inG Σ (authR (gsetUR (prodO locO locO)));
+  keys_name : gname;
+  keys_name2 : gname;
+}.
+
+
+Definition keysN := nroot .@ "keys".
+
+Section Keys.
+
+Context `{!heapG Σ, !cfgSG Σ, !keysSG Σ, !invG Σ}.
+
+Implicit Types bl : bool * loc.
+Implicit Types L : gsetUR (prodO boolO locO).
+Implicit Types LL : gsetUR (prodO locO locO).
+
+Definition keys_inv : iProp Σ :=
+  ∃ L LL,
+    own keys_name (● L) ∗ own keys_name2 (● LL)
+    ∗ ([∗ set] bl ∈ L, if bl.1 : bool then bl.2 ↦ #() else bl.2 ↦ₛ #())
+    ∗ ([∗ set] ll ∈ LL, ll.1 ↦ #() ∗ ll.2 ↦ₛ #()).
+
+Definition keys_ctx : iProp Σ :=
+  inv keysN keys_inv.
+
+End Keys.
+
+
+(* HACK: move somewhere else *)
+Ltac auto_equiv :=
+  (* Deal with "pointwise_relation" *)
+  repeat lazymatch goal with
+  | |- pointwise_relation _ _ _ _ => intros ?
+  end;
+  (* Normalize away equalities. *)
+  repeat match goal with
+  | H : _ ≡{_}≡ _ |-  _ => apply (discrete_iff _ _) in H
+  | H : _ ≡ _ |-  _ => apply leibniz_equiv in H
+  | _ => progress simplify_eq
+  end;
+  (* repeatedly apply congruence lemmas and use the equalities in the hypotheses. *)
+  try (f_equiv; fast_done || auto_equiv).
+
+Ltac solve_proper_alt :=
+  repeat intro; (simpl + idtac);
+  by repeat match goal with H : _ ≡{_}≡ _|- _ => rewrite H end.
+
+Ltac solve_proper ::= (repeat intros ?; simpl; auto_equiv).
+
+
+
+
+
+Definition logN : namespace := nroot .@ "logN".
+
+(** interp : is a unary logical relation. *)
+Section logrel.
+  Context `{heapG Σ, cfgSG Σ}.
+  Notation D := (prodO valO valO -n> iPropO Σ).
+  Implicit Types τi : D.
+  Implicit Types Δ : gmapO string D.
+  Implicit Types interp : gmapO string D -n> D.
+
+  Definition interp_expr (τi : gmapO string D -n> D) Δ
+      (ee : expr * expr) : iProp Σ := (∀ j K,
+    j ⤇ fill K (ee.2) →
+    WP ee.1 {{ v, ∃ v', j ⤇ fill K (of_val v') ∗ τi Δ (v, v') }})%I.
+  Global Instance interp_expr_ne n :
+    Proper (dist n ==> dist n ==> (=) ==> dist n) interp_expr.
+  Proof. unfold interp_expr; solve_proper. Qed.
+
+  Program Definition ctx_lookup (x : string) : gmapO string D -n> D := λne Δ,
+    from_option id (cconst True)%I (Δ !! x).
+  Solve Obligations with solve_proper.
+
+  Program Definition interp_unit : gmapO string D -n> D := λne Δ ww,
+    (⌜ww.1 = #()⌝ ∧ ⌜ww.2 = #()⌝)%I.
+  Solve Obligations with solve_proper_alt.
+  Program Definition interp_nat : gmapO string D -n> D := λne Δ ww,
+    (∃ n : nat, ⌜ww.1 = #n⌝ ∧ ⌜ww.2 = #n⌝)%I.
+  Solve Obligations with solve_proper.
+
+  Program Definition interp_bool : gmapO string D -n> D := λne Δ ww,
+    (∃ b : bool, ⌜ww.1 = #b⌝ ∧ ⌜ww.2 = #b⌝)%I.
+  Solve Obligations with solve_proper.
+
+  Program Definition interp_prod
+      interp1 interp2 : gmapO string D -n> D := λne Δ ww,
+    (∃ vv1 vv2, ⌜ww = (PairV (vv1.1) (vv2.1), PairV (vv1.2) (vv2.2))⌝ ∧
+                interp1 Δ vv1 ∧ interp2 Δ vv2)%I.
+  Solve Obligations with solve_proper.
+
+  Program Definition interp_sum
+      interp1 interp2 : gmapO string D -n> D := λne Δ ww,
+    ((∃ vv, ⌜ww = (InjLV (vv.1), InjLV (vv.2))⌝ ∧ interp1 Δ vv) ∨
+     (∃ vv, ⌜ww = (InjRV (vv.1), InjRV (vv.2))⌝ ∧ interp2 Δ vv))%I.
+  Solve Obligations with solve_proper.
+
+  Program Definition interp_arrow
+          interp1 interp2 : gmapO string D -n> D :=
+    λne Δ ww,
+    (□ ∀ vv, interp1 Δ vv →
+             interp_expr
+               interp2 Δ (App (of_val (ww.1)) (of_val (vv.1)),
+                          App (of_val (ww.2)) (of_val (vv.2))))%I.
+  Solve Obligations with solve_proper.
+
+  Program Definition interp_ref_inv (ll : loc * loc) : D -n> iPropO Σ := λne τi,
+    (∃ vv, ll.1 ↦ vv.1 ∗ ll.2 ↦ₛ vv.2 ∗ τi vv)%I.
+  Solve Obligations with solve_proper.
+
+  Program Definition interp_ref
+      interp : gmapO string D -n> D := λne Δ ww,
+    (∃ ll : loc * loc, ⌜ww = (#ll.1, #ll.2)⌝ ∧
+           inv (logN .@ ll) (interp_ref_inv ll (interp Δ)))%I.
+  Solve Obligations with solve_proper.
+
+  Fixpoint interp (τ : type) : listO D -n> D :=
+    match τ return _ with
+    | TUnit => interp_unit
+    | TNat => interp_nat
+    | TBool => interp_bool
+    | TProd τ1 τ2 => interp_prod (interp τ1) (interp τ2)
+    | TSum τ1 τ2 => interp_sum (interp τ1) (interp τ2)
+    | TArrow τ1 τ2 => interp_arrow (interp τ1) (interp τ2)
+    | TVar x => ctx_lookup x
+    | TForall τ' => interp_forall (interp τ')
+    | TRec τ' => interp_rec (interp τ')
+    | Tref τ' => interp_ref (interp τ')
+    end.
+  Notation "⟦ τ ⟧" := (interp τ).
+
+  Definition interp_env (Γ : list type)
+      (Δ : listO D) (vvs : list (val * val)) : iProp Σ :=
+    (⌜length Γ = length vvs⌝ ∗ [∗] zip_with (λ τ, ⟦ τ ⟧ Δ) Γ vvs)%I.
+  Notation "⟦ Γ ⟧*" := (interp_env Γ).
+
+  Class env_Persistent Δ :=
+    ctx_persistentP : Forall (λ τi, ∀ vv, Persistent (τi vv)) Δ.
+  Global Instance ctx_persistent_nil : env_Persistent [].
+  Proof. by constructor. Qed.
+  Global Instance ctx_persistent_cons τi Δ :
+    (∀ vv, Persistent (τi vv)) → env_Persistent Δ → env_Persistent (τi :: Δ).
+  Proof. by constructor. Qed.
+  Global Instance ctx_persistent_lookup Δ x vv :
+    env_Persistent Δ → Persistent (ctx_lookup x Δ vv).
+  Proof. intros HΔ; revert x; induction HΔ=>-[|?] /=; apply _. Qed.
+  Global Instance interp_persistent τ Δ vv :
+    env_Persistent Δ → Persistent (⟦ τ ⟧ Δ vv).
+  Proof.
+    revert vv Δ; induction τ=> vv Δ HΔ; simpl; try apply _.
+    rewrite /Persistent fixpoint_interp_rec1_eq /interp_rec1 /= intuitionistically_into_persistently.
+    by apply persistently_intro'.
+  Qed.
+  Global Instance interp_env_base_persistent Δ Γ vs :
+  env_Persistent Δ → TCForall Persistent (zip_with (λ τ, ⟦ τ ⟧ Δ) Γ vs).
+  Proof.
+    intros HΔ. revert vs.
+    induction Γ => vs; simpl; destruct vs; constructor; apply _.
+  Qed.
+  Global Instance interp_env_persistent Γ Δ vvs :
+    env_Persistent Δ → Persistent (⟦ Γ ⟧* Δ vvs) := _.
+
+  Lemma interp_weaken Δ1 Π Δ2 τ :
+    ⟦ τ.[upn (length Δ1) (ren (+ length Π))] ⟧ (Δ1 ++ Π ++ Δ2)
+    ≡ ⟦ τ ⟧ (Δ1 ++ Δ2).
+  Proof.
+    revert Δ1 Π Δ2. induction τ=> Δ1 Π Δ2; simpl; auto.
+    - intros ww; simpl; properness; auto. by apply IHτ1. by apply IHτ2.
+    - intros ww; simpl; properness; auto. by apply IHτ1. by apply IHτ2.
+    - unfold interp_expr.
+      intros ww; simpl; properness; auto. by apply IHτ1. by apply IHτ2.
+    - apply fixpoint_proper=> τi ww /=.
+      properness; auto. apply (IHτ (_ :: _)).
+    - rewrite iter_up; destruct lt_dec as [Hl | Hl]; simpl.
+      { by rewrite !lookup_app_l. }
+      (* FIXME: Ideally we wouldn't have to do this kinf of surgery. *)
+      change (bi_ofeO (uPredI (iResUR Σ))) with (uPredO (iResUR Σ)).
+      rewrite !lookup_app_r; [|lia ..]. do 2 f_equiv. lia.
+    - unfold interp_expr.
+      intros ww; simpl; properness; auto. by apply (IHτ (_ :: _)).
+    - intros ww; simpl; properness; auto. by apply IHτ.
+  Qed.
+
+  Lemma interp_subst_up Δ1 Δ2 τ τ' :
+    ⟦ τ ⟧ (Δ1 ++ interp τ' Δ2 :: Δ2)
+    ≡ ⟦ τ.[upn (length Δ1) (τ' .: ids)] ⟧ (Δ1 ++ Δ2).
+  Proof.
+    revert Δ1 Δ2; induction τ=> Δ1 Δ2; simpl; auto.
+    - intros ww; simpl; properness; auto. by apply IHτ1. by apply IHτ2.
+    - intros ww; simpl; properness; auto. by apply IHτ1. by apply IHτ2.
+    - unfold interp_expr.
+      intros ww; simpl; properness; auto. by apply IHτ1. by apply IHτ2.
+    - apply fixpoint_proper=> τi ww /=.
+      properness; auto. apply (IHτ (_ :: _)).
+    - rewrite iter_up; destruct lt_dec as [Hl | Hl]; simpl.
+      { by rewrite !lookup_app_l. }
+      (* FIXME: Ideally we wouldn't have to do this kinf of surgery. *)
+      change (bi_ofeO (uPredI (iResUR Σ))) with (uPredO (iResUR Σ)).
+      rewrite !lookup_app_r; [|lia ..].
+      case EQ: (x - length Δ1) => [|n]; simpl.
+      { symmetry. asimpl. apply (interp_weaken [] Δ1 Δ2 τ'). }
+      change (bi_ofeO (uPredI (iResUR Σ))) with (uPredO (iResUR Σ)).
+      rewrite !lookup_app_r; [|lia ..]. do 2 f_equiv. lia.
+    - unfold interp_expr.
+      intros ww; simpl; properness; auto. apply (IHτ (_ :: _)).
+    - intros ww; simpl; properness; auto. by apply IHτ.
+  Qed.
+
+  Lemma interp_subst Δ2 τ τ' v : ⟦ τ ⟧ (⟦ τ' ⟧ Δ2 :: Δ2) v ≡ ⟦ τ.[τ'/] ⟧ Δ2 v.
+  Proof. apply (interp_subst_up []). Qed.
+
+  Lemma interp_env_length Δ Γ vvs : ⟦ Γ ⟧* Δ vvs ⊢ ⌜length Γ = length vvs⌝.
+  Proof. by iIntros "[% ?]". Qed.
+
+  Lemma interp_env_Some_l Δ Γ vvs x τ :
+    Γ !! x = Some τ → ⟦ Γ ⟧* Δ vvs ⊢ ∃ vv, ⌜vvs !! x = Some vv⌝ ∧ ⟦ τ ⟧ Δ vv.
+  Proof.
+    iIntros (?) "[Hlen HΓ]"; iDestruct "Hlen" as %Hlen.
+    destruct (lookup_lt_is_Some_2 vvs x) as [v Hv].
+    { by rewrite -Hlen; apply lookup_lt_Some with τ. }
+    iExists v; iSplit. done. iApply (big_sepL_elem_of with "HΓ").
+    apply elem_of_list_lookup_2 with x.
+    rewrite lookup_zip_with; by simplify_option_eq.
+  Qed.
+
+  Lemma interp_env_nil Δ : ⊢ ⟦ [] ⟧* Δ [].
+  Proof. iSplit; simpl; auto. Qed.
+  Lemma interp_env_cons Δ Γ vvs τ vv :
+    ⟦ τ :: Γ ⟧* Δ (vv :: vvs) ⊣⊢ ⟦ τ ⟧ Δ vv ∗ ⟦ Γ ⟧* Δ vvs.
+  Proof.
+    rewrite /interp_env /= (assoc _ (⟦ _ ⟧ _ _)) -(comm _ ⌜(_ = _)⌝%I) -assoc.
+    by apply sep_proper; [apply pure_proper; lia|].
+  Qed.
+
+  Lemma interp_env_ren Δ (Γ : list type) vvs τi :
+    ⟦ subst (ren (+1)) <$> Γ ⟧* (τi :: Δ) vvs ⊣⊢ ⟦ Γ ⟧* Δ vvs.
+  Proof.
+    apply sep_proper; [apply pure_proper; by rewrite fmap_length|].
+    revert Δ vvs τi; induction Γ=> Δ [|v vs] τi; csimpl; auto.
+    apply sep_proper; auto. apply (interp_weaken [] [τi] Δ).
+  Qed.
+
+  Lemma interp_ref_pointsto_neq E Δ τ l w (l1 l2 l3 l4 : loc) :
+    ↑logN.@(l1, l2) ⊆ E →
+    l2 ≠ l4 →
+    l ↦ᵢ w -∗ interp (Tref τ) Δ (LocV l1, LocV l2) -∗
+      |={E ∖ ↑logN.@(l3, l4)}=> l ↦ᵢ w ∗ ⌜l ≠ l1⌝.
+  Proof.
+    intros Hnin Hneq.
+    destruct (decide (l = l1)); subst; last auto.
+    iIntros "Hl1"; simpl; iDestruct 1 as ((l5, l6)) "[% Hl2]"; simplify_eq.
+    iInv (logN.@(l5, l6)) as "Hi" "Hcl"; simpl.
+    iDestruct "Hi" as ((v1, v2))  "(Hl3 & Hl2' & ?)".
+    iMod "Hl3".
+    by iDestruct (@mapsto_valid_2 with "Hl1 Hl3") as %?.
+  Qed.
+
+  Lemma interp_ref_pointsto_neq' E Δ τ l w (l1 l2 l3 l4 : loc) :
+    ↑logN.@(l1, l2) ⊆ E →
+    l1 ≠ l3 →
+    l ↦ₛ w -∗ interp (Tref τ) Δ (LocV l1, LocV l2) -∗
+      |={E ∖ ↑logN.@(l3, l4)}=> l ↦ₛ w ∗ ⌜l ≠ l2⌝.
+  Proof.
+    intros Hnin Hneq.
+    destruct (decide (l = l2)); subst; last auto.
+    iIntros "Hl1"; simpl; iDestruct 1 as ((l5, l6)) "[% Hl2]"; simplify_eq.
+    iInv (logN.@(l5, l6)) as "Hi" "Hcl"; simpl.
+    iDestruct "Hi" as ((v1, v2)) "(Hl3 & >Hl2' & ?)".
+    by iDestruct (mapstoS_valid_2 with "Hl1 Hl2'") as %[].
+  Qed.
+
+  Lemma interp_ref_open' Δ τ l l' :
+    env_Persistent Δ → EqType τ →
+    ⟦ Tref τ ⟧ Δ (LocV l, LocV l') -∗
+               |={⊤, ⊤ ∖ ↑logN.@(l, l')}=>
+  ∃ w w', ▷ l ↦ᵢ w ∗ ▷ l' ↦ₛ w' ∗ ▷ ⟦ τ ⟧ Δ (w, w') ∗
+            ▷ (∀ z z' u u' v v',
+                  l ↦ᵢ z -∗ l' ↦ₛ z' -∗ ⟦ τ ⟧ Δ (u, u') -∗ ⟦ τ ⟧ Δ (v, v') -∗
+                    |={⊤ ∖ ↑logN.@(l, l')}=> l ↦ᵢ z ∗
+                                              l' ↦ₛ z' ∗ ⌜v = u ↔ v' = u'⌝)
+            ∗ (▷ (∃ vv : val * val, l ↦ᵢ vv.1 ∗ l' ↦ₛ vv.2 ∗ ⟦ τ ⟧ Δ vv)
+          ={⊤ ∖ ↑logN.@(l, l'), ⊤}=∗ True).
+  Proof.
+    iIntros (HΔ Heqt); simpl.
+    iDestruct 1 as ((l1, l1')) "[% H1]"; simplify_eq.
+    iInv (logN.@(l1, l1')) as "Hi" "$"; simpl.
+    iDestruct "Hi" as ((v1, v2))  "(Hl1 & Hl1' & Hrl)"; simpl in *.
+    destruct Heqt; simpl in *.
+    - iModIntro; iExists _, _; iFrame.
+      iNext. iIntros (??????) "? ?". iIntros ([??] [??]); subst.
+      by iModIntro; iFrame.
+    - iModIntro; iExists _, _; iFrame.
+      iNext. iIntros (??????) "? ?".
+      iDestruct 1 as (?) "[% %]". iDestruct 1 as (?) "[% %]".
+      simplify_eq. by iModIntro; iFrame.
+    - iModIntro; iExists _, _; iFrame.
+      iNext. iIntros (??????) "? ?".
+      iDestruct 1 as (?) "[% %]". iDestruct 1 as (?) "[% %]".
+      simplify_eq. by iModIntro; iFrame.
+    - iModIntro; iExists _, _; iFrame; iFrame "#". iNext.
+      iIntros (z z' u u' v v') "Hl1 Hl1' Huu". iDestruct 1 as ((l2, l2')) "[% #Hl2]";
+        simplify_eq; simpl in *.
+      iDestruct "Huu" as ((l3, l3')) "[% #Hl3]";
+        simplify_eq; simpl in *.
+      destruct (decide ((l1, l1') = (l2, l2'))); simplify_eq.
+      + destruct (decide ((l2, l2') = (l3, l3'))); simplify_eq; first by iFrame.
+        destruct (decide (l2 = l3)); destruct (decide (l2' = l3')); subst.
+        * iMod (interp_ref_pointsto_neq with "Hl1 []")
+               as "[Hl1 %]"; simpl; eauto.
+             by iFrame.
+        * iMod (interp_ref_pointsto_neq with "Hl1 []")
+               as "[Hl1 %]"; simpl; eauto.
+             { by iExists (_, _); iFrame "#". }
+             by iFrame.
+        * iMod (interp_ref_pointsto_neq' with "Hl1' []")
+               as "[Hl1' %]";
+               simpl; eauto.
+             { by iExists (_, _); iFrame "#". }
+             by iFrame.
+        * iFrame; iModIntro; iPureIntro; split; by inversion 1.
+      + destruct (decide ((l1, l1') = (l3, l3'))); simplify_eq.
+        * destruct (decide (l2 = l3)); destruct (decide (l2' = l3')); subst.
+          -- iMod (interp_ref_pointsto_neq with "Hl1 []")
+              as "[Hl1 %]"; simpl; eauto.
+             by iFrame.
+          -- iMod (interp_ref_pointsto_neq with "Hl1 []")
+               as "[Hl1 %]"; simpl; eauto.
+             { iExists (_, _); iSplit; first eauto. iFrame "#". }
+             by iFrame.
+          -- iMod (interp_ref_pointsto_neq' with "Hl1' []")
+               as "[Hl1' %]";
+               simpl; eauto.
+             { iExists (_, _); iSplit; first eauto. iFrame "#". }
+             by iFrame.
+          -- iFrame; iModIntro; iPureIntro; split; by inversion 1.
+        * destruct (decide ((l2, l2') = (l3, l3'))); simplify_eq.
+          -- destruct (decide (l1 = l3)); destruct (decide (l1' = l3')); subst.
+             ++ iMod (interp_ref_pointsto_neq with "Hl1 []")
+                 as "[Hl1 %]"; simpl; eauto.
+                by iFrame.
+             ++ iMod (interp_ref_pointsto_neq with "Hl1 []")
+               as "[Hl1 %]"; simpl; eauto.
+                { by iExists (_, _); iFrame "#". }
+                  by iFrame.
+             ++ iMod (interp_ref_pointsto_neq' with "Hl1' []")
+                 as "[Hl1' %]";
+                  simpl; eauto.
+                { by iExists (_, _); iFrame "#". }
+                  by iFrame.
+             ++ iFrame; iModIntro; iPureIntro; split; by inversion 1.
+          -- iFrame.
+             { destruct (decide (l2 = l3)); destruct (decide (l2' = l3'));
+                 simplify_eq; auto.
+               + iInv (logN.@(l3, l2')) as "Hib1" "Hcl1".
+                 iInv (logN.@(l3, l3')) as "Hib2" "Hcl2".
+                 iDestruct "Hib1" as ((v11, v12)) "(Hlx1' & Hlx2 & Hr1)".
+                 iDestruct "Hib2" as ((v11', v12')) "(Hl1'' & Hl2' & Hr2)".
+                 simpl.
+                 iMod "Hlx1'"; iMod "Hl1''".
+                   by iDestruct (@mapsto_valid_2 with "Hlx1' Hl1''") as %?.
+               + iInv (logN.@(l2, l3')) as "Hib1" "Hcl1".
+                 iInv (logN.@(l3, l3')) as "Hib2" "Hcl2".
+                 iDestruct "Hib1" as ((v11, v12)) "(>Hl1 & >Hl2' & Hr1)".
+                 iDestruct "Hib2" as ((v11', v12')) "(>Hl1' & >Hl2'' & Hr2) /=".
+                 by iDestruct (mapstoS_valid_2 with "Hl2' Hl2''") as %[].
+               + iModIntro; iPureIntro; split; intros; simplify_eq. }
+  Qed.
+End logrel.
+
+Typeclasses Opaque interp_env.
+Notation "⟦ τ ⟧" := (interp τ).
+Notation "⟦ τ ⟧ₑ" := (interp_expr (interp τ)).
+Notation "⟦ Γ ⟧*" := (interp_env Γ).
